disk-betree/Mkfs.i.dfy
@@ -11,54 +11,39 @@ module {:extern} MkfsImpl {
   import BT = PivotBetreeSpec
   import BC = BetreeGraphBlockCache
   import ReferenceType`Internal
-  import LBAType`Internal
+  import LBAType
   import ValueWithDefault`Internal
   import IS = ImplState
   import D = AsyncDisk
 
   type LBA = LBAType.LBA
 
-  method InitDisk() returns (result: map<LBA, IS.Sector>)
-  ensures forall k | k in result :: IS.WFSector(result[k])
-  ensures forall l | l in result :: result[l].SectorBlock? ==> BT.WFNode(IS.INode(result[l].block))
-  ensures forall l | l in result :: result[l].SectorBlock? ==> Marshalling.CappedNode(result[l].block)
-  ensures 0 in result && result[0].SectorIndirectionTable?
-  ensures LBAType.BlockSize() in result && result[LBAType.BlockSize()].SectorBlock?
-  {
-    var sectorIndirectionTable := new IS.MutIndirectionTable(1024); // TODO magic number
-    assume sectorIndirectionTable.Count == 0;
-    var _ := sectorIndirectionTable.Insert(0, (Some(LBAType.BlockSize()), []));
-    assert IS.IIndirectionTable(sectorIndirectionTable) == BC.IndirectionTable(map[0 := LBAType.BlockSize()], map[0 := []]);
-    result := map[
-      // Map ref 0 to lba 1
-      0 := IS.SectorIndirectionTable(sectorIndirectionTable),
-      // Put the root at lba 1
-      LBAType.BlockSize() := IS.SectorBlock(IS.Node([], None, [KMTable.Empty()]))
-    ];
-
-    assume Marshalling.CappedNode(IS.SectorBlock(IS.Node([], None, [KMTable.Empty()])).block);
-
-    assume forall k | k in result :: IS.WFSector(result[k]);
-  }
-
   // TODO spec out that the data returned by this function
   // satisfies the initial conditions
   // TODO prove that this always returns an answer (that is, marshalling always succeeds)
   method InitDiskBytes() returns (m :  map<LBA, array<byte>>)
-  //ensures forall lba | lba in m :: ValidSector(m[lba][..])
   {
-    var d := InitDisk();
+    assume Marshalling.CappedNode(IS.SectorBlock(IS.Node([], None, [KMTable.Empty()])).block);
+    var b1 := Marshalling.MarshallCheckedSector(IS.SectorBlock(IS.Node([], None, [KMTable.Empty()])));
 
-    LBAType.reveal_ValidAddr();
+    var sectorIndirectionTable := new IS.MutIndirectionTable(1024); // TODO magic number
+    assume sectorIndirectionTable.Count == 0;
+    var _ := sectorIndirectionTable.Insert(0, (Some(LBAType.Location(LBAType.BlockSize(), b1.Length as uint64)), []));
+    assert IS.IIndirectionTable(sectorIndirectionTable) == BC.IndirectionTable(
+      map[0 := LBAType.Location(LBAType.BlockSize(), b1.Length as uint64)],
+      map[0 := []]
+    );
 
-    assert d[0].SectorIndirectionTable?;
-    var b0 := Marshalling.MarshallCheckedSector(d[0]);
-    if (b0 == null) { return map[]; }
+    assume IS.WFSector(IS.SectorIndirectionTable(sectorIndirectionTable));
+    var b0 := Marshalling.MarshallCheckedSector(IS.SectorIndirectionTable(sectorIndirectionTable));
+    assume b0 != null;
 
-    assert d[LBAType.BlockSize()].SectorBlock?;
-    var b1 := Marshalling.MarshallCheckedSector(d[LBAType.BlockSize()]);
-    if (b1 == null) { return map[]; }
+    m := map[
+      // Map ref 0 to lba 1
+      0 := b0,
+      // Put the root at lba 1
+      LBAType.BlockSize() := b1
+    ];
 
-    m := map[0 := b0, LBAType.BlockSize() := b1];
   }
 }
